Rearranged everything, added comments

stlc-norm.fst
@@ -2,6 +2,85 @@ module StlcNormalizing
 
 open StlcCbvDbParSubst
 open Constructive
+
+(*** Facts about substitution and closedness *)
+val id : sub
+let id (x : var) = EVar x
+                        
+val subst_id : e:exp -> Lemma (subst id e = e)
+let rec subst_id e = using_induction_hyp subst_id
+
+val update : sub -> var -> exp -> Tot sub                        
+let update s x v y = if y = x then v else s y
+type closed (e : exp) = (forall y. not(appears_free_in y e))
+type closed2 (sigma:sub) = (forall x. sigma x <> EVar x ==> closed(sigma x))
+
+val closed_app : e1 : exp -> e2:exp -> Lemma (requires (closed (EApp e1 e2))) (ensures (closed e1 /\ closed e2))
+let closed_app = admit() (* intuitively trivial *)                                             
+                    
+val subst_closed : e:exp -> 
+   Lemma (requires (closed e)) (ensures (forall sigma. subst sigma e = e))
+let rec subst_closed e =
+  match e with
+  | EApp e1 e2 -> closed_app e1 e2; subst_closed e1; subst_closed e2
+  | ELam t1 e1 -> admit() (* needs work, or different definition of closedness *)
+
+val substitution_lemma' : #g:env -> g':env -> #e:exp -> #t:typ -> sigma:sub ->
+                          typing g e t ->
+                          (x:var -> t:typ -> g'':env -> Tot (typing g'' (sigma x) t)
+                                                            (requires (g x == Some t /\ sigma x <> EVar x))
+                                                            (ensures True)) ->
+                          (x:var -> t:typ -> Lemma (requires (g x == Some t /\ sigma x == EVar x))
+                                                   (ensures (g' x == Some t))) ->
+                          Tot (typing g' (subst sigma e) t)
+let rec substitution_lemma' g g' e t sigma ty_g h1 h2 =
+  match ty_g with
+  | TyVar x -> if sigma x <> EVar x then h1 x t g' else (h2 x t; TyVar x)
+  | TyApp #g_ #e1 #e2 ih1 ih2 -> TyApp (substitution_lemma' g' sigma ih1 h1 (fun x t -> h2 x t)) (substitution_lemma' g' sigma ih2 h1 (fun x t -> h2 x t))
+  | TyLam #g t1 #e1 #t2 ih1 ->
+     TyLam t1 (substitution_lemma' (extend g' 0 t1) (subst_elam sigma) ih1 (magic()) (fun x t -> admit()))
+
+val invariance_env : #e:exp -> #t:typ -> g:env -> g':env -> typing g e t -> Tot (typing g' e t) (requires (forall x. is_Some (g x) ==> g x == g' x)) (ensures True)
+let rec invariance_env e t g g' ty_g =
+  match ty_g with
+  | TyApp ty_arrow ty_arg -> TyApp (invariance_env g g' ty_arrow) (invariance_env g g' ty_arg)
+  | TyLam argT ty_ext -> TyLam argT (invariance_env (extend g 0 argT) (extend g' 0 argT) ty_ext)
+  | TyVar #g x -> magic()
+
+val invariance_empty : #e:exp -> #t:typ ->
+  typing empty e t -> g:env -> Tot ( typing g e t )
+let invariance_empty e t ty g = invariance_env #e #t empty g ty
+                                   
+val substitution_lemma : #g:env -> g':env -> #e:exp -> #t:typ -> sigma:sub ->
+                         typing g e t ->
+                         (x:var -> t:typ -> Tot (cexists (fun e -> h:(typing empty e t){g x == Some t ==> sigma x == e}))) ->
+                         Tot (typing g' (subst sigma e) t)
+let rec substitution_lemma g g' e t sigma ty_g h2 =                             
+  substitution_lemma' g' sigma ty_g (fun x t g'' -> match h2 x t with
+                                                      ExIntro s h -> let (u:unit{g x == Some t}) = magic() in
+                                                                     invariance_empty h g'')
+                      (fun x t -> match h2 x t with ExIntro s h -> ())       
+
+
+val subst_update : x:var -> v:exp -> e:exp -> sigma:sub{closed2 sigma} ->
+                   Lemma (subst_beta v (subst (subst_elam sigma) e) = subst (update (subst_elam sigma) 0 v) e)
+let rec subst_update x v e sigma = match e with
+  | EVar x -> if x > 0 then
+                (
+                  if (sigma (x-1) <> EVar (x-1)) then
+                    (
+                      assert(closed (sigma (x-1)));
+                      subst_closed (sigma(x-1))
+                    )
+                  else
+                    (
+                      admit() (* this should hold per definition *)
+                    )
+                )
+  | EApp e1 e2 -> subst_update x v e1 sigma; subst_update x v e2 sigma
+  | _ -> admit()                      
+                      
+(*** Evaluation and halting terms *)                       
        
 kind Relation (a:Type) = a -> a -> Type
 type multi (a:Type) (r:Relation a) : a -> a -> Type =
@@ -10,40 +89,9 @@ type multi (a:Type) (r:Relation a) : a -> a -> Type =
 type steps : exp -> exp -> Type = fun x y -> multi exp step x y
 type halts (e:exp) : Type = cexists (fun e' -> u:(steps e e'){is_value e'})
 
-(* This has a negative occurrence of R that makes Coq succumb,
-although this definition is just fine (the type decreases);
-F* should have similar problems as soon as we start checking
-for negative occurrences. Hopefully by then we will also have
-a solution for this. *)
-type red : typ -> exp -> Type =
-| R_bool :  #e:exp -> typing empty e TBool -> halts e -> red TBool e
-| R_arrow : t1:typ -> t2:typ -> #e:exp ->
-            typing empty e (TArr t1 t2) ->
-            halts e ->
-            (e':exp -> red t1 e' -> Tot (red t2 (EApp e e'))) ->
-            red (TArr t1 t2) e
-(*                
-| R_pair : t1:typ -> t2:typ -> e:exp{typing empty e (TPair t1 t2) ->
-           halts e ->
-           red t1 (EFst e) ->
-           red t2 (ESnd e) ->
-           red (TPair t1 t2) e
- *)                
-                
+                                    
 val value_normal : v:exp{is_value v} -> Tot (halts v)
 let value_normal v = match v with ELam _ _ -> ExIntro v (Multi_refl v)
-                
-val red_halts : #t:typ -> #e:exp -> red t e -> Tot (halts e)
-let red_halts t e h =
-  match h with
-  | R_arrow _ _ _ hh _ -> hh
-  | R_bool _ hh -> hh
-                                                           
-val red_typable_empty : #t:typ -> #e:exp -> red t e -> Tot (typing empty e t)
-let red_typable_empty t e h =
-  match h with
-  | R_arrow k1 k2 ht k3 k4 -> ht
-  | R_bool t_e ht -> t_e
 
 val step_deterministic : e:exp -> e':exp -> e'':exp -> step e e' -> step e e'' -> Lemma (e' = e'')
 let rec step_deterministic e e' e'' step1 step2 =
@@ -71,7 +119,6 @@ let rec step_deterministic e e' e'' step1 step2 =
       | SApp1 #fe1 fe2 #fe1' fstep_e -> ()
       | SBeta argT' body' arg' -> ()
      )
-									    
 
 val step_preserves_halting : e:exp -> e':exp -> step e e' -> Tot (ciff (halts e) (halts e'))           
 let rec step_preserves_halting e e' s_e_e' =
@@ -86,6 +133,35 @@ let rec step_preserves_halting e e' s_e_e' =
      match h with ExIntro v to_v -> ExIntro v (Multi_step e e' v s_e_e' to_v)
   in                                          
     Conj p1 p2
+
+       
+(*** The relation red *)                                                      
+
+(* This has a negative occurrence of R that makes Coq succumb,
+although this definition is just fine (the type decreases);
+F* should have similar problems as soon as we start checking
+for negative occurrences. Hopefully by then we will also have
+a solution for this. *)
+type red : typ -> exp -> Type =
+| R_bool :  #e:exp -> typing empty e TBool -> halts e -> red TBool e
+| R_arrow : t1:typ -> t2:typ -> #e:exp ->
+            typing empty e (TArr t1 t2) ->
+            halts e ->
+            (e':exp -> red t1 e' -> Tot (red t2 (EApp e e'))) ->
+            red (TArr t1 t2) e       
+                
+val red_halts : #t:typ -> #e:exp -> red t e -> Tot (halts e)
+let red_halts t e h =
+  match h with
+  | R_arrow _ _ _ hh _ -> hh
+  | R_bool _ hh -> hh
+                                                           
+val red_typable_empty : #t:typ -> #e:exp -> red t e -> Tot (typing empty e t)
+let red_typable_empty t e h =
+  match h with
+  | R_arrow k1 k2 ht k3 k4 -> ht
+  | R_bool t_e ht -> t_e
+
 
 val step_preserves_red : e:exp -> e':exp -> step e e' -> t:typ -> red t e ->
 				     Tot (red t e') (decreases t)
@@ -137,84 +213,15 @@ let rec step_preserves_red' e e' s_e_e' t ty_t h =
       | R_bool t_e ht ->
 	 let p : (halts e) = match (step_preserves_halting e e' s_e_e') with Conj pa pb -> pb ht in
 	 R_bool ty_t p
-     )
-
-val steps_preserves_red' : e:exp -> e':exp -> steps e e' -> t:typ -> typing empty e t -> red t e' -> Tot (red t e) (decreases t)         
-let rec steps_preserves_red' e e' s_e_e' t ty_t h = admit()
+     )                       
+                                        
+(*** The relations red2 and ered *)                       
 
 type red2 (g:env) (sigma:sub) =
     cand (x : var -> t : typ -> Tot (cexists (fun e -> h:(red t e){g x == Some t ==> sigma x == e})))
          (x : var -> e : exp -> Tot (cexists (fun t -> h:(red t e){sigma x == e /\ EVar x <> e ==> g x == Some t})))
-                
-(* Definition R' (Gamma:ctx) (theta:sub) : Prop := *)
-(* (forall x S, Gamma x = Some S -> exists s, theta x = Some s /\ R S s) *)
-(* /\ *)
-(* (forall x s, theta x = Some s -> exists S, Gamma x = Some S /\ R S s). *)
-(* type closed2 (sigma:sub) = (forall x e.sigma x = e /\ x <> e ==> closed e) *)
+type ered (t : typ) (e : exp) = e':exp -> step e e' -> Tot (red t e')
 
-(* val red_closed2 : sigma:sub -> g:env -> red2 g sigma -> Tot (closed'                              *)
-
-(* Lemma R_implies_closed': forall theta Gamma, *)
-(*   R' Gamma theta -> closed' theta.                              *)
-
-val substitution_lemma' : #g:env -> g':env -> #e:exp -> #t:typ -> sigma:sub ->
-                          typing g e t ->
-                          (x:var -> t:typ -> g'':env -> Tot (typing g'' (sigma x) t)
-                                                            (requires (g x == Some t /\ sigma x <> EVar x))
-                                                            (ensures True)) ->
-                          (x:var -> t:typ -> Lemma (requires (g x == Some t /\ sigma x == EVar x))
-                                                   (ensures (g' x == Some t))) ->
-                          Tot (typing g' (subst sigma e) t)
-let rec substitution_lemma' g g' e t sigma ty_g h1 h2 =
-  match ty_g with
-  | TyVar x -> if sigma x <> EVar x then h1 x t g' else (h2 x t; TyVar x)
-  | TyApp #g_ #e1 #e2 ih1 ih2 -> TyApp (substitution_lemma' g' sigma ih1 h1 (fun x t -> h2 x t)) (substitution_lemma' g' sigma ih2 h1 (fun x t -> h2 x t))
-  | TyLam #g t1 #e1 #t2 ih1 ->
-     TyLam t1 (substitution_lemma' (extend g' 0 t1) (subst_elam sigma) ih1 (magic()) (fun x t -> admit()))
-
-val invariance_env : #e:exp -> #t:typ -> g:env -> g':env -> typing g e t -> Tot (typing g' e t) (requires (forall x. is_Some (g x) ==> g x == g' x)) (ensures True)
-let rec invariance_env e t g g' ty_g =
-  match ty_g with
-  | TyApp ty_arrow ty_arg -> TyApp (invariance_env g g' ty_arrow) (invariance_env g g' ty_arg)
-  | TyLam argT ty_ext -> TyLam argT (invariance_env (extend g 0 argT) (extend g' 0 argT) ty_ext)
-  | TyVar #g x -> magic()
-
-val invariance_empty : #e:exp -> #t:typ ->
-  typing empty e t -> g:env -> Tot ( typing g e t )
-let invariance_empty e t ty g = invariance_env #e #t empty g ty
-
-
-(*
- | TyVar : #g:env ->
-            x:var{is_Some (g x)} ->
-            typing g (EVar x) (Some.v (g x))
-  | TyLam : #g:env ->
-            t:typ ->
-            #e1:exp ->
-            #t':typ ->
-            typing (extend g 0 t) e1 t' ->
-            typing g (ELam t e1) (TArr t t')
-  | TyApp : #g:env ->
-            #e1:exp ->
-            #e2:exp ->
-            #t11:typ ->
-            #t12:typ ->
-            typing g e1 (TArr t11 t12) ->
-            typing g e2 t11 ->
-            typing g (EApp e1 e2) t12
-
-*)
-                                   
-val substitution_lemma : #g:env -> g':env -> #e:exp -> #t:typ -> sigma:sub ->
-                         typing g e t ->
-                         (x:var -> t:typ -> Tot (cexists (fun e -> h:(typing empty e t){g x == Some t ==> sigma x == e}))) ->
-                         Tot (typing g' (subst sigma e) t)
-let rec substitution_lemma g g' e t sigma ty_g h2 =                             
-  substitution_lemma' g' sigma ty_g (fun x t g'' -> match h2 x t with
-                                                      ExIntro s h -> let (u:unit{g x == Some t}) = magic() in
-                                                                     invariance_empty h g'')
-                      (fun x t -> match h2 x t with ExIntro s h -> ())                      
-                      
 val red_subst : g:env -> e:exp -> t:typ -> sigma:sub ->
                 typing g e t ->
                 red2 g sigma ->
@@ -224,33 +231,11 @@ let red_subst g e t sigma ty_t r = substitution_lemma empty sigma ty_t
                                          let Conj r1 r2 = r in
                                          let ExIntro s h1 = r1 x t in
                                          ExIntro s (red_typable_empty h1))
-
-type ered (t : typ) (e : exp) = e':exp -> step e e' -> Tot (red t e')
-
-(* val red_term_ap : t1:typ -> t2:typ -> e:exp{not (is_value e)} -> *)
-(*                   (u:exp -> typing empty u t2 -> ered t2 u -> *)
-(*                    Tot (red t2 u) (requires (not (is_value u))) (ensures True)) -> *)
-(*                   typing empty e (TArr t1 t2) -> *)
-(*                   ered (TArr t1 t2) e -> *)
-(*                   e':exp -> red t1 e' -> v:exp{is_value v} -> steps e' v -> Tot( red t2 (EApp e e')) *)
-(* let red_term_ap t1 t2 e f ty_e ered_e e' red_e' v h =  *)
-(*   let rec induction (h : steps e' v) (h4 : red t1 e') : (\* Tot *\) (red t2 (EApp e e')) =  *)
-(*     match h with *)
-(*     | Multi_refl _ -> magic() *)
-(*     | Multi_step e1 e2 e3 s_e_e2 st_e2_e' -> *)
-(*        f (EApp e e') (TyApp ty_e (red_typable_empty h4)) *)
-(*          (fun u (s_u : step (EApp e e') u) ->  *)
-(*           match s_u with *)
-(*           | SApp1 e2 #e1 s_e_e1 -> *)
-(*              let hh : step e e1 = s_e_e1 in *)
-(*              (match ered_e e1 hh with *)
-(*                 R_arrow n1 n2 n3 n4 g -> g e' red_e' ) *)
-(*           | SApp2 _ _ -> magic() *)
-(*          ) *)
-(*   in *)
-(*   (\* induction h red_e' *\) magic() *)
-
-
+val red2_preserves_update :
+    #g:env -> #sigma:sub -> t:typ -> u:exp ->
+    red2 g sigma -> Tot ( red2 (extend g 0 t) (update (subst_elam sigma) 0 u) )
+let red2_preserves_update = magic()                             
+                     
 val red_exp_closed : #t:typ -> e:exp{not (is_value e)} ->
                      typing empty e t ->
                      ered t e ->
@@ -258,8 +243,6 @@ val red_exp_closed : #t:typ -> e:exp{not (is_value e)} ->
 let red_exp_closed t e ty_t f =
   let ExIntro e' h = progress ty_t in
   step_preserves_red' e e' h t ty_t (f e' h)
-
-
 
 val red_beta_induction : t1:typ -> t2:typ -> e:exp ->
                typing (extend empty 0 t1) e t2 ->
@@ -292,19 +275,14 @@ val red_beta : t1:typ -> t2:typ -> e:exp ->
 let red_beta t1 t2 e ty_t2 f e' red_e' =
   let ExIntro v steps_e'v = red_halts red_e' 
   in red_beta_induction t1 t2 e ty_t2 f e' red_e' v steps_e'v
+                                                                
 
-val update : sub -> var -> exp -> Tot sub                        
-let update s x v y = if y = x then v else s y
+val red2_closed' : #g : env -> #sigma : sub ->
+                   red2 g sigma -> Lemma (closed2 sigma)
+let red2_closed' = admit()
 
-                                            
-val red2_preserves_update :
-    #g:env -> #sigma:sub -> t:typ -> u:exp ->
-    red2 g sigma -> Tot ( red2 (extend g 0 t) (update (subst_elam sigma) 0 u) )
-let red2_preserves_update = magic()                                            
-                        
-val subst_update : x:var -> v:exp -> e:exp -> sigma:sub ->
-                   Lemma (subst_beta v (subst (subst_elam sigma) e) = subst (update (subst_elam sigma) 0 v) e)
-let subst_update = admit()
+
+(*** The main lemma and the final theorem *)
                         
 val main :
       e:exp -> #t:typ -> #t':typ -> #g:env -> sigma:sub ->
@@ -330,6 +308,7 @@ let rec main e t t' g sigma red2_g ty_t =
         assert (subst sigma e == ELam t1 (subst (subst_elam sigma) e1));
         let p : (typing (extend empty 0 t1) (e1') t2) = (match b with TyLam bla h4 -> h4) in
         let f : (u:exp -> red t1 u -> Tot (red t2 (subst_beta u e1'))) = fun u red_u ->
+          red2_closed' red2_g;
           subst_update 0 u e1 sigma;
           assert (subst_beta u e1' = subst (update (subst_elam sigma) 0 u) e1);
           let r : (red2 (extend g 0 t1) (update (subst_elam sigma) 0 u)) = red2_preserves_update t1 u red2_g in
@@ -340,23 +319,12 @@ let rec main e t t' g sigma red2_g ty_t =
        R_arrow t1 t2 #(subst sigma e) b ex (f)
 
 
-val id : sub
-let id (x : var) = EVar x
-                        
-val subst_id : e:exp -> Lemma (subst id e = e)
-let rec subst_id e = using_induction_hyp subst_id
-
+(* This may help to prove the following fact *)
 assume val exfalso_quodlibet : unit -> Tot 'a (requires (False)) (ensures True)
                                          
 val red2_id_empty : red2 empty id
 let red2_id_empty = magic()
 
-(* type red2 (g:env) (sigma:sub) = *)
-(*     cand (x : var -> t : typ -> 
-             Tot (cexists (fun e -> h:(red t e){g x == Some t ==> sigma x == e}))) *)
-(*          (x : var -> e : exp -> 
-             Tot (cexists (fun t -> h:(red t e){sigma x == e /\ EVar x <> e ==> g x == Some t}))) *)
-			 
 val normalization :
       #e:exp -> #t:typ ->
       typing empty e t ->
